mrdts-new/Set-wins_map/App_new.fst
@@ -1,6 +1,7 @@
 module App_new
 
 module S = Set_extended
+module M = Map_extended
 
 #set-options "--query_stats"
 
@@ -114,11 +115,7 @@ let rc_base (l:concrete_st) (o o1 o2:op_t)
           
 let rc_base_base (o1 o2:op_t)
   : Lemma (requires distinct_ops o1 o2 /\ Fst_then_snd? (rc o1 o2))
-          (ensures eq (merge init_st (do init_st o1) (do init_st o2)) (do (do init_st o1) o2)) = 
-  let lhs = (merge init_st (do init_st o1) (do init_st o2)) in
-  let rhs = (do (do init_st o1) o2) in
-  //assert (forall k. M.contains lhs k = M.contains rhs k);
-  ()
+          (ensures eq (merge init_st (do init_st o1) (do init_st o2)) (do (do init_st o1) o2)) = ()
 
 let rc_intermediate_base_right (l s1 s2 s3:concrete_st) (o o' o1 o2:op_t) 
   : Lemma (requires distinct_ops o o' /\ Fst_then_snd? (rc o o') /\ 
@@ -127,6 +124,14 @@ let rc_intermediate_base_right (l s1 s2 s3:concrete_st) (o o' o1 o2:op_t)
                     eq (merge l (do s1 o1) (do s2 o2)) (do (do s3 o1) o2) /\
                     eq (merge l (do s1 o') (do s2 o)) (do (do s3 o) o')) //***EXTRA***
           (ensures eq (merge (do l o') (do (do s1 o') o1) (do (do (do s2 o) o') o2)) (do (do (do (do s3 o) o') o1) o2)) = ()
+
+let rc_intermediate_base_left (l s1 s2 s3:concrete_st) (o o' o1 o2:op_t) 
+  : Lemma (requires distinct_ops o o' /\ Fst_then_snd? (rc o o') /\ 
+                    distinct_ops o1 o2 /\ Fst_then_snd? (rc o1 o2) /\
+                    eq (merge (do l o') (do (do s1 o') o1) (do (do s2 o') o2)) (do (do (do s3 o') o1) o2) /\
+                    eq (merge l (do s1 o1) (do s2 o2)) (do (do s3 o1) o2) /\
+                    eq (merge l (do s1 o') (do s2 o)) (do (do s3 o) o')) //***EXTRA***
+          (ensures eq (merge (do l o') (do (do (do s1 o) o') o1) (do (do s2 o') o2)) (do (do (do (do s3 o) o') o1) o2)) = admit()
           
 let rc_intermediate_base_left_right (l s1 s2 s3:concrete_st) (o o' o1' o1 o2:op_t) 
   : Lemma (requires distinct_ops o o' /\ Fst_then_snd? (rc o o') /\  
@@ -330,3 +335,33 @@ let comm_intermediate_1_v1 (l s1 s2 s3:concrete_st) (o1 o2 o:op_t)
                     (exists o'. Fst_then_snd? (rc o' o)) /\
                     eq (merge l (do s1 o1) (do s2 o2)) (do (do s3 o1) o2))
           (ensures eq (merge (do l o) (do (do s1 o) o1) (do (do s2 o) o2)) (do (do (do s3 o) o1) o2)) = ()
+
+////////////////////////////////////////////////////////////////
+//// Sequential implementation //////
+
+// the concrete state 
+type concrete_st_s = M.t nat nat
+
+// init state 
+let init_st_s = M.const 0
+
+// apply an operation to a state 
+let do_s (s:concrete_st_s) (op:op_t) : concrete_st_s = 
+  match op with
+  |(_, (_, Set k v)) -> M.upd s k v //S.add (k,v) s 
+  |(_, (_, Del k)) -> M.del s k //S.filter s (fun e -> fst (snd e) <> k)
+
+//equivalence relation between the concrete states of sequential type and MRDT
+let eq_sm (st_s:concrete_st_s) (st:concrete_st) = 
+  admit()
+
+//initial states are equivalent
+let initial_eq _
+  : Lemma (ensures eq_sm init_st_s init_st) = admit()
+
+//equivalence between states of sequential type and MRDT at every operation
+let do_eq (st_s:concrete_st_s) (st:concrete_st) (op:op_t)
+  : Lemma (requires eq_sm st_s st)
+          (ensures eq_sm (do_s st_s op) (do st op)) = admit()
+
+////////////////////////////////////////////////////////////////
